$$
\delta _j ^l = \frac{\partial C}{\partial z_j^l} = \sum _k \frac{\partial C}{\partial z_k ^{l+1}}\cdot \frac{\partial z_k^{l+1}}{\partial a_j^l }\cdot \frac{\partial a_j^l}{\partial z_j^l}
\\ = \sum_{k=1} \delta_k^{l+1} \cdot \frac{\partial (w_{kj}^{l+1}a_j^l+b_k^{l+1})}{\partial a_j^{l+1}} \cdot \sigma ' (z_j ^l)
\\ = \sum_{k} \delta_k^{l+1} \cdot w_{kj}^{l+1} \cdot \sigma ' (z_j^l)
\\ \delta^l  = ((w^{l+1})^T\delta ^{l+1}) \odot \sigma ' (z^l)
\\ \frac{\partial C}{\partial w_{jk}^l} = a_k^{l-1}\delta_j^l
\\ \frac{\partial C}{\partial w_{jk}^l} =\frac{\partial C}{\partial z_j^{l}} \cdot \frac{\partial z_j^l}{\partial w_{jk} ^l} = \delta_j^l \cdot \frac{\partial (w_{jk}^la_{k}^{l-1}b_j^l)}{\partial w_{jk}^l} =a_k^{l-1}\delta_j^l
\\ \frac{\partial C}{\partial b_j^l} = \delta_j^l
\\ \frac{\partial C}{\partial b_j^l} =\frac{\partial C}{\partial z_j^{l}} \cdot \frac{\partial z_j^l}{\partial b_j ^l} = \delta_j^l \cdot \frac{\partial (w_{jk}^la_{k}^{l-1}b_j^l)}{\partial b_j^l} =\delta_j^l
\\ w^l \rightarrow w^l - \frac{\eta}{m}\sum_{x}\delta^{x,l}(a^{x,l-1})^T
\\ b^l \rightarrow b^l - \frac{\eta}m \sum_x \delta^{x,l}
\\D_x = \frac{1}{n}\{ \sum_{i=1}^n |BFS_j| - |BFS_{j-1}|\}
\\H_{td} = -\sum_{i=1}^n P_{tdi}\log_2 P_{tdi} \ \ \ \ \ \ \ \ i\in \{1,2,3 \cdots\}
\\H_t = \sum_{d=1}^D H_{td}
\\ f(x) = \omega^T x + b
\\ r_t = \sigma (W_r\cdot[h_{t-1},x_t] + b_r)
\\ z_t = \sigma (W_z \cdot [h_{i-1},x_t] + b_z)
\\ \overline {h_t} = \tanh (W \cdot [r_i \cdot h_{i-1},x_t] + b)
\\ h_t = (1-z_t) \cdot h_{i-1} + z \cdot \overline{h_t}
\\ RMSE = \sqrt{\frac{1}{N}\sum_{i=1}^N (y_i - \widetilde{y_i})}
\\ MAE = \frac{1}{N}\sum_{i=1}^N |y_i - \widetilde{y_i}|
\\ MAPE(y,\widehat{y}) = \frac{\sum_{i=1}^n |\frac{y_i - \widehat{y_i}}{y_i}|}{n} \times 100\%
\\ MAPE(y,\widehat{y}) = \frac{\sum_{i=1}^n |\frac{y_i - \widehat{y_i}}{y_i}|}{n} \times 100\%
\\\widehat{y} = w^T \varphi(x) + b
\\ \widehat{y} = \sum_{i=1}^N \alpha _iK(x,x_i) + b
\\ X'(t) = X(t) + w_i(t),
\ \ \ \ \ \ \ \ i\in \{1,2,3 \cdots\}
\\ X'(t) = \sum_{j=1}^J C_{i,j}(t) + r_i(t)
\\  \{ \{ C_{1,1}(t), C_{2,1}(t), \cdots ,C_{n,1}(t) \} ,\cdots , \{ C_{1,j}(t), C_{2,j}(t), \cdots ,C_{n,j}(t)\} \}
\\ C_{j}(t) = \frac{1}{n}\sum_{i=1}^n C_{i,j}(t)
\ \ \ \ \ \ \ \ j\in \{1,2, \cdots ,J\}
\\r(t) = \frac{1}{n}\sum_{i=1}^n r_i(t)
\\MSE = (\frac{1}{L}\sum_{i=1}^L(\widehat{y_i} - y_i^{m + 1}))^2
\\d_t = f_t - f_{t-1}
\ \ \ \ \ \ \ \ t \in \{2, \cdots ,n\}
\\V_x = \sum_{r=1}^p w_rD_r
\\d_t = f_{t+1} - f_t
\\f_{new} = f_i + d_t\cdot rand(0,1)
\\P_{tdits} = \frac{BFS_{tdits}}{U_{tdits}}
\ \ \ \ \ \ \ \ t\in \{ 1,2,3,\cdots , m\}
\\S = \{(x_1,y_1),\cdots ,(x_i,y_i), \cdots ,(x_m,y_m) \}
\ \ \ \ \ \ \ \ y_i\in \{-1,1\},x \in \mathbb{R}^n
\\f_t = \sigma(W_f[h_{t-1},x_t] + b_f)
\\fi_t = \sigma(W_i[h_{t-1},x_t] + b_i)
\\ \overline{c_t} = \tanh(W_c[h_{t-1},x_t] + b_c)
\\c_t = f_t \odot c_{t-1} + i_t \odot \overline{c_t}
\\o_t = \sigma(W_o[h_{t-1},x_t] + b_o)
\\h_t = o_t \odot \tanh(c_t)
\\R^2 = \frac{\sum_{i=1}^N (y_i - \widetilde{y_i})(\widehat{y_i} - \widehat{\widetilde{y_i}})}{\sqrt{\sum_{i=1}^N(y_i - \widetilde{y_i})^2}\sqrt{\sum_{i=1}^N (\widehat{y_i} - \widehat{\widetilde{y_i}})^2}}
\\fs_{(i,j)} = ft_{(i,j)} + fp_{(i,j)}+fr_{(i,j)}
\\\begin{bmatrix} 0 & -1 \\ 1 & 0 \end{bmatrix}
$$